@prefix : <https://linked.data.gov.au/def/gsq/dataset#> .
@prefix owl: <http://www.w3.org/2002/07/owl#> .
@prefix rdf: <http://www.w3.org/1999/02/22-rdf-syntax-ns#> .
@prefix xml: <http://www.w3.org/XML/1998/namespace> .
@prefix xsd: <http://www.w3.org/2001/XMLSchema#> .
@prefix dcat: <http://www.w3.org/ns/dcat#> .
@prefix prof: <http://www.w3.org/ns/dx/prof/> .
@prefix rdfs: <http://www.w3.org/2000/01/rdf-schema#> .
@base <https://linked.data.gov.au/def/gsq/dataset> .

<https://linked.data.gov.au/def/gsq/dataset> rdf:type owl:Ontology ;
                                             owl:versionIRI <https://linked.data.gov.au/def/gsq-dataset/> ;
                                             owl:imports <http://www.w3.org/2006/time#2016> ,
                                                         <http://www.w3.org/ns/dcat> ,
                                                         <http://www.w3.org/ns/sosa/> ,
                                                         <http://www.w3.org/ns/ssn/ext> ;
                                             <http://purl.org/dc/elements/1.1/creator> "Nicholas J. Car" ;
                                             <http://purl.org/dc/elements/1.1/publisher> "Geological Survey of Queensland" ;
                                             <http://purl.org/dc/terms/created> "2019-04-03"^^xsd:date ;
                                             <http://purl.org/dc/terms/creator> <http://orcid.org/0000-0002-8742-7730> ;
                                             <http://purl.org/dc/terms/modified> "2019-04-03"^^xsd:date ;
                                             <http://purl.org/dc/terms/publisher> <http://catalogue.linked.data.gov.au/org/gsq> ;
                                             rdfs:comment "This ontology is the Geological Survey of Queensland (GSQ)'s profile of the Dataset Catalogue Vocabulary, DCAT. It implements GSQ-specific constraints on the use of DCAT to ensure that datasets catalogues by GSQ contain certain properties that GSQ requires."@en ;
                                             rdfs:label "GSQ Dataset Profile" ;
                                             owl:versionInfo "See the GitHub repo https://github.com/geological-survey-of-queensland/gsq-dataset-profile for versioning"@en .

#################################################################
#    Annotation properties
#################################################################

###  http://www.w3.org/2002/07/owl#qualifiedCardinality
owl:qualifiedCardinality rdf:type owl:AnnotationProperty .


#################################################################
#    Object Properties
#################################################################

###  https://linked.data.gov.au/def/gsq/dataset/hadGenerationMethod
<https://linked.data.gov.au/def/gsq/dataset/hadGenerationMethod> rdf:type owl:ObjectProperty ;
                                                                rdfs:domain dcat:Dataset ;
                                                                rdfs:range <http://www.w3.org/2004/02/skos/core#Concept> ;
                                                                owl:propertyChainAxiom ( <http://www.w3.org/ns/prov#wasGeneratedBy>
                                                                                         <http://www.w3.org/ns/prov#qualifiedAssociation>
                                                                                         <http://www.w3.org/ns/prov#hadPlan>
                                                                                       ) ;
                                                                rdfs:label "This property links a Sample or a Dataset to a Procedure or a Method which may be expressed as a skos:Concept" ,
                                                                           "had generation method" .


#################################################################
#    Classes
#################################################################

###  https://linked.data.gov.au/def/gsq/dataset/CrustalSample
<https://linked.data.gov.au/def/gsq/dataset/CrustalSample> rdf:type owl:Class ;
                                                          rdfs:subClassOf <http://www.w3.org/ns/sosa/Sample> ,
                                                                          [ rdf:type owl:Restriction ;
                                                                            owl:onProperty <http://www.w3.org/ns/ssn/ext/hasUltimateFeatureOfInterest> ;
                                                                            owl:qualifiedCardinality "1"^^xsd:nonNegativeInteger ;
                                                                            owl:onClass <https://linked.data.gov.au/def/gsq/dataset/EarthsCrustFOI>
                                                                          ] ;
                                                          rdfs:comment "A Sample who's ultimate Feature of Interest is a Feature of Interest within the Earth's Crust."@en ;
                                                          rdfs:label "Crustal Sample" .


###  https://linked.data.gov.au/def/gsq/dataset/EarthsCrustFOI
<https://linked.data.gov.au/def/gsq/dataset/EarthsCrustFOI> rdf:type owl:Class ;
                                                           rdfs:subClassOf <http://www.w3.org/ns/sosa/FeatureOfInterest> ;
                                                           rdfs:comment "A Feature of Interest within the Earth's Crust, that is within the outermost solid shell of the Earth with the following two depth-from-surface ranges: Oceanic: 5 km to 10 km and and composed primarily of denser, more mafic rocks, such as basalt, diabase, and gabbro and Continental: 30 km to 50 km and mostly composed of less dense, more felsic rocks, such as granite."@en ;
                                                           rdfs:label "Earth's Crust Feature of Interest"@en .


###  https://linked.data.gov.au/def/gsq/dataset/SamplingDataset
<https://linked.data.gov.au/def/gsq/dataset/SamplingDataset> rdf:type owl:Class ;
                                                            rdfs:subClassOf dcat:Dataset ,
                                                                            <http://www.w3.org/ns/sosa/Sample> ,
                                                                            [ rdf:type owl:Restriction ;
                                                                              owl:onProperty <http://www.w3.org/ns/sosa/isResultOf> ;
                                                                              owl:qualifiedCardinality "1"^^xsd:nonNegativeInteger ;
                                                                              owl:onClass <http://www.w3.org/ns/sosa/Sampling>
                                                                            ] ;
                                                            rdfs:comment "Sampling Datasets are Datasets that are the result of Sampling activities. The Sampling could be of any sort - active seismic sampling, satellite imaging etc. The main feature of a Sampling Dataset is that it is both a Dataset within a catalogue and also a Sample from a sensor."@en ;
                                                            rdfs:label "Sampling Dataset" .


###  https://linked.data.gov.au/def/gsq/dataset/SeismicSamplingDataset
<https://linked.data.gov.au/def/gsq/dataset/SeismicSamplingDataset> rdf:type owl:Class ;
                                                                   rdfs:subClassOf <https://linked.data.gov.au/def/gsq/dataset/SamplingDataset> ;
                                                                   rdfs:comment "Seismic Sampling datasets are Sampling Datasets that are the results of Seismic Sampling events. They necissarily have a seismic sampling method as their procedure."@en ;
                                                                   rdfs:label "Seismic Sampling Dataset"@en .


###  https://linked.data.gov.au/def/gsq/dataset/SeismicSamplingProcedure
<https://linked.data.gov.au/def/gsq/dataset/SeismicSamplingProcedure> rdf:type owl:Class ;
                                                                     rdfs:subClassOf <http://www.w3.org/ns/sosa/Procedure> .


###  http://org.semanticweb.owlapi/error#Error3
<http://org.semanticweb.owlapi/error#Error3> rdf:type owl:Class .


###  http://org.semanticweb.owlapi/error#Error4
<http://org.semanticweb.owlapi/error#Error4> rdf:type owl:Class .


###  http://www.w3.org/ns/dcat#Dataset
dcat:Dataset rdfs:subClassOf <http://org.semanticweb.owlapi/error#Error3> ,
                             <http://org.semanticweb.owlapi/error#Error4> ,
                             [ rdf:type owl:Restriction ;
                               owl:onProperty <http://www.w3.org/2006/time#hasTime> ;
                               owl:allValuesFrom <http://www.w3.org/2006/time#TemporalEntity>
                             ] ,
                             [ rdf:type owl:Restriction ;
                               owl:onProperty dcat:contactPoint ;
                               owl:qualifiedCardinality "1"^^xsd:nonNegativeInteger ;
                               owl:onClass <http://purl.org/dc/terms/Agent>
                             ] .


[ owl:qualifiedCardinality "1"^^xsd:nonNegativeInteger
] .

[ owl:qualifiedCardinality "1"^^xsd:nonNegativeInteger
 ] .

###  Generated by the OWL API (version 4.5.6.2018-09-06T00:27:41Z) https://github.com/owlcs/owlapi
